progress in proof

NTCB/ValidatorProof.v
@@ -12,7 +12,8 @@ Require Import Validator.
 
 Module ValProof (Import I : INSTRUCTION) (Import ISP: INSTRUCTION_SEMANTICS_PROP(I)).
   Module Val := ValidatorCode(I).
-
+  Module ProgSem := Prog_Semantics(I).
+  Import ProgSem.
   Import Val.
   Ltac fun_ind_validate_n_byte :=
     match goal with
@@ -120,6 +121,291 @@ Module ValProof (Import I : INSTRUCTION) (Import ISP: INSTRUCTION_SEMANTICS_PROP
     validate_ll_list_increase_valid_addresses.
 
 
+  Lemma validate_n_byte_add_addr:
+    forall (addr: N) n
+    (valid_addresses to_be_checked_addresses: NSet) (ll: lazy_list byte)
+    valid_addresses' to_be_checked_addresses' ll',
+    validate_n_byte (S n) None addr valid_addresses to_be_checked_addresses ll =
+    Some (valid_addresses', to_be_checked_addresses', ll') ->
+    In_NSet addr valid_addresses'.
+  Proof.
+    intros * VALIDATE.
+    functional inversion VALIDATE; subst;
+    subst;
+    repeat match goal with
+      | x := _ : _ |- _ => subst x
+    end;
+    apply validate_n_byte_increase_valid_addresses in X;
+    eauto with nset.
+  Qed.
+
+  Local Hint Resolve validate_n_byte_add_addr.
+
+  Lemma validate_n_byte_size: 
+    forall (n: nat) (oreg: option register) (addr: N)
+    (valid_addresses to_be_checked_addresses: NSet) (ll: lazy_list byte)
+    valid_addresses' to_be_checked_addresses',
+    validate_n_byte n oreg addr valid_addresses to_be_checked_addresses ll =
+    Some (valid_addresses', to_be_checked_addresses', 〈〉) ->
+    ll_length ll = n.
+  Proof.
+    intros * VALIDATE.
+    fun_ind_validate_n_byte; clean;
+    specialize (IHo VALIDATE); subst;
+    apply ll_safe_drop_size in e2;
+    apply safe_minus_correct in e3; omega.
+  Qed.
+
+  Ltac omega' := zify; omega.
+
+  Lemma addresses_multiple_of_32_in_valid_addresses:
+    forall addr valid_addresses to_be_checked_addresses ll
+      valid_addresses' to_be_checked_addresses',
+      dividable_by_32 addr ->
+      validate_ll_list addr valid_addresses to_be_checked_addresses ll =
+        Some (valid_addresses', to_be_checked_addresses') ->
+      forall addr', addr <= addr' -> addr' < addr + (N_of_nat (ll_length ll)) ->
+        dividable_by_32 addr' -> In_NSet addr' valid_addresses'.
+  Proof.
+    intros *.
+    fun_ind_validate_ll; intros; clean; eauto.
+    Case "fun_ind_validate_ll 1".
+      pose proof (validate_n_byte_size _ _ _ _ _ _ _ _ e).
+      apply validate_n_byte_add_addr in e.
+      replace addr' with addr. assumption.
+      rewrite H0 in H2. simpl in H2.
+      destruct H. destruct H3. zify. omega.
+
+    Case "fun_ind_validate_ll 2".
+      assert (dividable_by_32 (addr + 32)).
+        destruct H. exists (x + 1). zify; omega.
+        specialize (IHo H4 H0).
+        destruct (N_eq_dec addr addr').
+        SCase "addr = addr'".
+          subst.
+          eapply validate_ll_list_increase_valid_addresses; eauto.
+        SCase "addr <> addr'".
+          destruct H as [xaddr H].
+          destruct H3 as [xaddr' H3]. subst.
+          apply IHo. omega'.
+          replace 32 with (N_of_nat 32) by reflexivity.
+          rewrite <- Nplus_assoc. rewrite <- N_of_plus. 
+          erewrite <- ll_safe_drop_size; eauto.
+          exists xaddr'; eauto.
+  Qed.
+
+
+  Definition one_step_correct code_size
+    valid_addresses to_be_checked_addresses st1 :=
+    (~step header_size code_size st1 DANGER_STATE) /\
+    forall st2, step header_size code_size st1 (Normal_state st2) ->
+    (  dividable_by_32 st2.(state_pc) 
+    \/ In_NSet st2.(state_pc) valid_addresses
+    \/ In_NSet st2.(state_pc) to_be_checked_addresses).
+    
+  Definition two_steps_correct code_size
+    valid_addresses to_be_checked_addresses st1 :=
+    (~step header_size code_size st1 DANGER_STATE) /\
+    forall st2, step header_size code_size st1 (Normal_state st2) ->
+    (  dividable_by_32 st2.(state_pc) 
+    \/ In_NSet st2.(state_pc) valid_addresses
+    \/ In_NSet st2.(state_pc) to_be_checked_addresses
+    \/ one_step_correct code_size valid_addresses
+         to_be_checked_addresses st2).
+
+  Lemma one_step_correct_trans:
+    forall code_size valid_addresses valid_addresses'
+      to_be_checked_addresses to_be_checked_addresses' st,
+      Nincluded to_be_checked_addresses to_be_checked_addresses' ->
+      Nincluded valid_addresses valid_addresses' ->
+      one_step_correct code_size valid_addresses
+        to_be_checked_addresses st ->
+      one_step_correct code_size valid_addresses'
+        to_be_checked_addresses' st.
+  Proof.
+    unfold one_step_correct, Nincluded.
+    intuition eauto.
+    edestruct H3 as [ | [ |]]; eauto.
+  Qed.
+
+  Hint Resolve one_step_correct_trans.
+
+  Lemma two_steps_correct_trans:
+    forall code_size valid_addresses valid_addresses'
+      to_be_checked_addresses to_be_checked_addresses' st,
+      Nincluded to_be_checked_addresses to_be_checked_addresses' ->
+      Nincluded valid_addresses valid_addresses' ->
+      two_steps_correct code_size valid_addresses
+        to_be_checked_addresses st ->
+      two_steps_correct code_size valid_addresses'
+        to_be_checked_addresses' st.
+  Proof.
+    unfold two_steps_correct, Nincluded.
+    intuition eauto.
+    edestruct H3 as [ | [ |[|]]]; eauto.
+  Qed.
+
+
+      
+
+  Definition memory_compat_addr_ll addr ll (mem: memory):=
+    forall n, (n < ll_length ll)%nat -> ll_nth n ll = mem (addr + N_of_nat n).
+
+
+  (* to lib *)
+  Lemma ll_safe_drop_nth {X}: forall n (ll: lazy_list X) ll',
+    ll_safe_drop n ll = Some ll' ->
+    forall i, ll_nth i ll' = ll_nth (n + i) ll.
+  Proof.
+    induction' n as [|n]; auto; simpl; intros; clean.
+    Case "S n".
+      destruct' ll as [|x [ll]]; clean.
+  Qed.
+      
+    
+
+
+  Lemma memory_compat_addr_ll_drop: forall addr ll mem n ll',
+    ll_safe_drop n ll = Some ll' ->
+    memory_compat_addr_ll addr ll mem ->
+    memory_compat_addr_ll (addr + N_of_nat n) ll' mem.
+  Proof.
+    unfold memory_compat_addr_ll. intros.
+    erewrite ll_safe_drop_nth; eauto.
+    rewrite <- Nplus_assoc. rewrite <- N_of_plus. apply H0.
+    apply ll_safe_drop_size in H. omega.
+  Qed.
+
+  Local Hint Resolve memory_compat_addr_ll_drop.
+
+(*  Lemma parse_instr_impl_read_instr:
+    forall ll instr size_instr
+  parse_instruction (byte_map_from_ll ll) = Some (instr, size_instr) ->
+  memory_compat_addr_ll addr ll mem ->
+  same_code (header_size + code_size) mem st.(state_mem) ->
+  in_code header_size code_size st ->
+  read_instr_from_memory st.(state_mem) st.(state_pc) = Some instr. *)
+
+  Ltac clean_safe_minus :=
+    repeat match goal with
+      | H : safe_minus _ _ = Some _ |- _ =>
+        apply safe_minus_correct in H
+           end.
+
+  Lemma validate_n_byte_two_steps: forall code_size (n: nat) (addr: N)
+    (valid_addresses to_be_checked_addresses: NSet) (ll: lazy_list byte)
+    valid_addresses' to_be_checked_addresses' ll',
+    validate_n_byte n None addr valid_addresses to_be_checked_addresses ll =
+      Some (valid_addresses', to_be_checked_addresses', ll') ->
+    addr + (N_of_nat n) <= header_size + code_size ->
+    forall mem, memory_compat_addr_ll addr ll mem ->
+    (forall addr', In_NSet addr' valid_addresses ->
+     forall st, same_code (header_size + code_size) mem st.(state_mem) ->
+       In_NSet st.(state_pc) valid_addresses ->
+       two_steps_correct code_size
+         valid_addresses to_be_checked_addresses st) ->
+    (forall addr', In_NSet addr' valid_addresses' ->
+     forall st, same_code (header_size + code_size) mem st.(state_mem) ->
+       In_NSet st.(state_pc) valid_addresses' ->
+       two_steps_correct code_size
+         valid_addresses' to_be_checked_addresses' st).
+  Proof.
+    intros *.
+    fun_ind_validate_n_byte; intros; clean; eauto;
+      eapply IHo0; clear IHo0; clean_safe_minus; eauto; try omega';
+        intros; clean; eauto;
+      (destruct (Nadd_In_or _ _ _ H8);
+        [(subst; clear H7)
+        | solve [eapply two_steps_correct_trans; eauto with nset]]).
+
+    Case "fun_ind_validate_n_byte 2".
+      unfold two_steps_correct.
+      constructor'.
+      NSCase "Non danger".
+        intro DANGER. 
+        inv DANGER.
+      assert (read_instr_from_memory st0.(state_mem) st0.(state_pc)
+                = Some (instr, size_instr)).
+        unfold read_instr_from_memory.
+        eapply parse_instruction_only_read; eauto.
+        unfold byte_map_from_ll. intros. unfold memory_compat_addr_ll in H0.
+        rewrite Nplus_comm. auto.
+   Admitted.
+      
+      
+
+  Lemma validate_ll_list_two_steps: forall code_size (addr: N)
+    (valid_addresses to_be_checked_addresses: NSet) (ll: lazy_list byte)
+    valid_addresses' to_be_checked_addresses',
+    validate_ll_list addr valid_addresses to_be_checked_addresses ll =
+      Some (valid_addresses', to_be_checked_addresses') ->
+    addr + (N_of_nat (ll_length ll)) <= header_size + code_size ->
+    forall mem, memory_compat_addr_ll addr ll mem ->
+    (forall addr', In_NSet addr' valid_addresses ->
+     forall st, same_code (header_size + code_size) mem st.(state_mem) ->
+       In_NSet st.(state_pc) valid_addresses ->
+       two_steps_correct code_size
+         valid_addresses to_be_checked_addresses st) ->
+    (forall addr', In_NSet addr' valid_addresses' ->
+     forall st, same_code (header_size + code_size) mem st.(state_mem) ->
+       In_NSet st.(state_pc) valid_addresses' ->
+       two_steps_correct code_size
+         valid_addresses' to_be_checked_addresses' st).
+  Proof.
+    intros *.
+    fun_ind_validate_ll; intros; clean; eauto.
+    Case "fun_ind_validate_ll 1".
+      eapply validate_n_byte_two_steps; eauto.
+      apply validate_n_byte_size in e. rewrite e in H0. auto.
+    Case "fun_ind_validate_ll 2".
+      eapply IHo; eauto; clear IHo.
+
+      apply validate_n_byte_drop_n in e. apply ll_safe_drop_size in e.
+      rewrite e in H0. rewrite N_of_plus in H0. simpl N_of_nat in H0.
+      omega'.
+
+      replace 32 with (N_of_nat 32) by reflexivity.
+      eapply memory_compat_addr_ll_drop; eauto.
+
+      intros. eapply validate_n_byte_two_steps; eauto.
+      apply validate_n_byte_drop_n in e. apply ll_safe_drop_size in e.
+      rewrite e in H0. rewrite N_of_plus in H0. simpl N_of_nat in H0.
+      omega'.
+  Qed.
+      
+
+  Theorem roxx: forall ll code_size valid_addresses to_be_checked_addresses,
+    validate_ll_list header_size Nempty Nempty ll = Some (valid_addresses, to_be_checked_addresses) ->
+    Nincluded to_be_checked_addresses valid_addresses ->
+    code_size = N_of_nat (ll_length ll) ->
+    forall mem, memory_compat_addr_ll header_size ll mem ->
+    forall st, same_code (header_size + code_size) mem st.(state_mem) ->
+      (In_NSet st.(state_pc) valid_addresses) ->
+      ~accessible_danger header_size code_size st.
+  Proof.
+    intros. intro.
+    revert H4 H3.
+    induction' H5; intros.
+    Case "AD_one_step".
+    assert (two_steps_correct code_size valid_addresses to_be_checked_addresses st1).
+      eapply validate_ll_list_two_steps; eauto.
+      omega'.
+      intros. apply Nempty_empty in H8. inv H8.
+    inv H6. apply H7. assumption.
+
+   Case "AD_more_steps".
+    assert (two_steps_correct code_size valid_addresses to_be_checked_addresses st1).
+      eapply validate_ll_list_two_steps; eauto.
+      omega'.
+      intros. apply Nempty_empty in H9. inv H9.
+    inv H7.
+
+
+(* toutes les addresses multiple de 32 sont dans valid_addresses
+
+
+
+ *)
 
 
 
